Seal for_postcondition

new/golang/theory/loop.v
@@ -5,6 +5,9 @@ From iris_named_props Require Export named_props.
 
 Set Default Proof Using "Type".
 
+(* See the documentation for the tactic [wp_for] below for an idea of the
+exported interface of this file. *)
+
 Section wps.
 Context `{ffi_sem: ffi_semantics} `{!ffi_interp ffi} `{!heapGS Σ}.
 
@@ -37,15 +40,17 @@ Proof.
   wp_call_lc "?". by iApply "Hwp".
 Qed.
 
-(* FIXME: seal this *)
-Definition for_postcondition stk E (post : val) P Φ bv : iProp Σ :=
+(* Sealed - use the wp_for_post_ lemmas below to prove this. *)
+Definition for_postcondition_def stk E (post : val) P Φ bv : iProp Σ :=
             ⌜ bv = continue_val ⌝ ∗ WP post #() @ stk; E {{ _, P }} ∨
             (∃ v, ⌜ bv = execute_val v ⌝ ∗ WP post #() @ stk; E {{ _, P }}) ∨
             ⌜ bv = break_val ⌝ ∗ Φ (execute_val #()) ∨
-            (∃ v, ⌜ bv = return_val v ⌝ ∗ Φ bv)
-.
+            (∃ v, ⌜ bv = return_val v ⌝ ∗ Φ bv).
+Definition for_postcondition_aux : seal (@for_postcondition_def). Proof. by eexists. Qed.
+Definition for_postcondition := (for_postcondition_aux).(unseal).
+Definition for_postcondition_eq : @for_postcondition = @for_postcondition_def  := (for_postcondition_aux).(seal_eq).
 
-Theorem wp_for P stk E (cond body post : val) Φ :
+Lemma wp_for P stk E (cond body post : val) Φ :
   P -∗
   □ (P -∗
      WP cond #() @ stk ; E {{ v, if decide (v = #true) then
@@ -59,6 +64,7 @@ Theorem wp_for P stk E (cond body post : val) Φ :
 Proof.
   iIntros "HP #Hloop".
   rewrite do_for_unseal.
+  rewrite for_postcondition_eq.
   iLöb as "IH".
   wp_call.
   iDestruct ("Hloop" with "HP") as "Hloop1".
@@ -112,26 +118,32 @@ Lemma wp_for_post_do (v : val) stk E (post : val) P Φ :
   WP (post #()) @ stk; E {{ _, P }} -∗
   for_postcondition stk E post P Φ (execute_val v).
 Proof.
-  iIntros "H". rewrite /for_postcondition. iRight. iLeft. iFrame "H". iPureIntro. by eexists.
+  iIntros "H". rewrite for_postcondition_eq /for_postcondition_def.
+  eauto 10 with iFrame.
 Qed.
 
 Lemma wp_for_post_continue stk E (post : val) P Φ :
   WP (post #()) @ stk; E {{ _, P }} -∗
   for_postcondition stk E post P Φ continue_val.
 Proof.
-  iIntros "H". rewrite /for_postcondition. iLeft. iFrame "H". iPureIntro. by eexists.
+  iIntros "H". rewrite for_postcondition_eq /for_postcondition_def.
+  eauto 10 with iFrame.
 Qed.
 
 Lemma wp_for_post_return stk E (post : val) P Φ v :
   Φ (return_val v) -∗
   for_postcondition stk E post P Φ (return_val v).
 Proof.
-  iIntros "H". rewrite /for_postcondition. repeat iRight. iExists _. iFrame "H". done.
+  iIntros "H". rewrite for_postcondition_eq /for_postcondition_def.
+  eauto 10 with iFrame.
 Qed.
 
 End wps.
 
-(** Tactic for convenient loop reasoning *)
+(** Tactic for convenient loop reasoning. First use [iAssert] to generalize the
+current context to the loop invariant, then apply this tactic. Use
+[wp_for_post_do], [wp_for_post_continue], and [wp_for_post_return] at the leaves
+of the proof. *)
 Ltac wp_for :=
   wp_bind (do_for _ _ _); iApply (wp_for with "[-]");
   [ by iNamedAccu
